examples/sbf/FilterRepr.v
@@ -1,0 +1,40 @@
+Require Import Coq.ZArith.BinInt.
+Require Import Coq.Strings.String.
+Require Import Poulet4.P4light.Semantics.Semantics.
+Require Import ProD3.examples.sbf.Utils.
+Require Import ProD3.examples.sbf.UseTofino.
+Require ProD3.examples.sbf.ConFilter.
+Require Import ProD3.examples.sbf.AbsFilter.
+Require Import ProD3.core.Coqlib.
+Require Import ProD3.core.ExtPred.
+Import ListNotations.
+Open Scope Z_scope.
+Open Scope string_scope.
+Open Scope list_scope.
+
+Section FilterRepr.
+
+Variable (p : path).
+
+Definition row_ge : genv -> Prop.
+Admitted.
+
+Definition row_inv_bare : extern_state -> Prop.
+Admitted.
+
+Lemma row_inv_wellformed : ep_wellformed_prop [p] row_inv_bare.
+Admitted.
+
+Definition row_inv : ext_pred :=
+  mk_ext_pred' row_inv_bare [p] row_inv_wellformed.
+
+Definition bool_to_val (b : bool) : ValueBase :=
+  ValBaseBit [b; false; false; false; false; false; false; false].
+
+Definition row_reg_repr (cr : ConFilter.row) : ext_pred :=
+  ExtPred.singleton (p ++ ["reg_row"]) (Tofino.ObjRegister (map bool_to_val cr)).
+
+Program Definition row_repr (cr : ConFilter.row) : ext_pred :=
+  ExtPred.wrap [p] (ExtPred.and row_inv (row_reg_repr cr)) _.
+Next Obligation.
+Admitted.
